\documentclass[main.tex]{subfiles}
\begin{document}

\section{Sheet 11}

\subsection{Wave equation}

\subsubsection{General travelling impulse}

We want to show that any twice-differentiable function \(F(z \pm v t) = f(z, t)\) solves the wave equation: 
%
\boxalign{
\begin{align} \label{eq:wave-equation}
\qty(-\partial_{t}^2 + v^2 \partial_{z}^2) f(t, z) = 0
\,. 
\end{align}}

We denote \(\alpha (t,z) = z \pm vt\), so that \(f = F \circ \alpha \) and: 
%
\begin{subequations}
\begin{align}
\pdv[2]{f}{t} = \pdv{}{t }\qty( \dv{F}{\alpha } \pdv{\alpha }{t}) &= \dv{F}{\alpha } \pdv[2]{\alpha }{t} +  \pdv{\alpha }{t} \pdv{}{t} \qty(\dv{F}{\alpha })  \\
&= \dv{F}{\alpha } \pdv[2]{\alpha }{t}
+ \pdv{\alpha }{t}\dv{}{\alpha } \qty(\dv{F}{\alpha } \pdv[]{\alpha }{t}) \marginnote{Commuted the derivatives}\\
&= \dv{F}{\alpha } \pdv[2]{\alpha }{t}
+ \pdv{\alpha }{t} \qty( \dv[2]{F}{\alpha } \pdv[]{\alpha }{t} 
+ \dv{F}{\alpha } \cancelto{}{\pdv{}{t} \dv{\alpha }{\alpha }}) \marginnote{Derivative of a constant}  \\
&= \dv{F}{\alpha } \pdv[2]{\alpha }{t}
+ \dv[2]{F}{\alpha } \qty(\pdv[]{\alpha }{t})^2  \label{eq:faa-di-bruno}\\
&= v^2 \dv[2]{F}{\alpha }
\,,
\end{align}
\end{subequations}
%
where the expression we derived is fully general up to equation \eqref{eq:faa-di-bruno}, while the last passage comes from the fact that \(\pdv*{\alpha }{t} = \pm v\), so its square is \(v^2\) while the second derivative is zero since \(v\) is a constant. By the same reasoning, 
%
\begin{subequations}
\begin{align}
\pdv[2]{f}{z} &= \dv{F}{\alpha } \pdv[2]{\alpha }{z} 
+ \dv[2]{F}{\alpha } \qty(\pdv{\alpha }{z})^2  \\
&= \dv[2]{F}{\alpha }
\,.
\end{align}
\end{subequations}

Therefore, 
%
\begin{align}
\qty(-\partial_{t}^2 + v^2 \partial_{z}^2) f(t, z) 
= (-v^2 + v^2) \dv[2]{F}{\alpha } \equiv 0 
\,.
\end{align}

\subsubsection{Gaussian pulse}

At any fixed time \(t\), the function 
%
\begin{align}
F(\alpha ) = \exp(- \alpha^2) = \exp(- \qty(z - v t)^2)
\,
\end{align}
%
looks like a rescaled Gaussian, centered around \(z = vt\). As \(t\) increases it travels rightward with speed \(v\). A plot of this, with \(v = 6\) and \(t = 0, 1, 2\) is shown in figure \ref{fig:moving-gaussian-pulse}.

\begin{figure}[H]
\centering
\includegraphics[width=\textwidth]{figures/gauss.pdf}
\caption{Pulse for \(t = 0, 1, 2\).}
\label{fig:moving-gaussian-pulse}
\end{figure}

\subsubsection{Harmonic wave solution}

We consider the harmonic solution 
%
\begin{align}
f(t,z) 
= A \cos(2 \pi \qty(\frac{z}{\lambda } - \frac{t}{T})) 
= A \cos(\frac{2\pi}{\lambda } \alpha (t,z)) 
\,,
\end{align}
%
where \(\alpha  = z - \lambda t /T\). Writing the harmonic solution this way allows us to see the properties easily: we have \(v  = \lambda / T\) by comparison with the formula from before (\(\alpha = z - vt\)), while the periodicity follows from that of the cosine: we start from the fact that \(\cos(x) = \cos(x \pm 2 \pi )\).

If we map \(z \rightarrow z  + \lambda \) we get \(\alpha \rightarrow \alpha +\lambda \), and 
%
\begin{align}
\cos(\frac{2 \pi }{\lambda } \alpha ) \rightarrow \cos(\frac{2 \pi }{\lambda }\qty(\alpha + \lambda )) = \cos(\frac{2 \pi }{\lambda } \alpha  + 2 \pi ) = \cos(\frac{2 \pi }{\lambda } \alpha )
\,.
\end{align}

Similarly, if we map \(t \rightarrow t + T\) we get \(\alpha \rightarrow \alpha - \lambda T/T = \alpha - \lambda  \), so we can apply the same reasoning. This means that the wave has spatial period \(\lambda \) and temporal period \(T\). 

\subsubsection{Lightspeed waves}

The equation \(\square f = 0\) is analogous to \eqref{eq:wave-equation} for \(v = 1 (= c)\). The difference is the three-dimensionality of the spatial derivatives, however this does not present an issue. 
We still consider solutions in the form \(f (x^{\mu }) = F(\alpha (x^{\mu }) )\), with \(\alpha (x^{\mu }) = k_{\mu } x^{ \mu }\) for a constant covector \(k_{\mu }\). We will have the following derivatives 
%
\begin{align}
\pdv[2]{f}{(x^{\mu })} 
= \dv[2]{F}{\alpha }
\qty( \pdv{\alpha }{(x^{\mu})} )^2
= \dv[2]{F}{\alpha }
\qty(k_{\mu })^2
\,,
\end{align}
%
where the index \(\mu \) can take the conventional values from \(0\) to \(3\). 
So, the equation \(\square f = 0\) reads 
%
\begin{align}
\dv[2]{F}{\alpha } \qty(-\qty(k_{0})^2 + \sum_{i=1 }^{3} \qty(k_{i })^2) = 0
\,,
\end{align}
%
which is always satisfied if we take for  \(k_{\mu }\) a null vector with respect to the Minkowski metric, \(k_{\mu } \eta^{\mu \nu } k_{\nu } = 0 \). 
In order for the wave to be propagating forwards in time we need to set \(k_{0} < 0\), or equivalently \(k^{0}>0\). 

So, the wave equation does indeed have travelling waves as solutions, which propagate with speed 1 (which can be gathered from the factor multiplying the Laplacian). 

\subsection{Gravitational waves}

\subsubsection{Weak-field wave equation}

We consider a perturbed metric \(g_{\mu \nu } = \eta_{\mu \nu } + h_{\mu \nu }\), to first order in \(h_{\mu \nu }\). 

First of all we need to compute the Christoffel symbols: they are given by 
%
\begin{subequations}
\begin{align}
\Gamma^{\mu }_{\nu \rho } 
&= \frac{1}{2} g^{\mu \alpha } \qty(g_{\alpha \nu , \rho } + g_{\alpha \rho , \nu } - g_{\nu \rho , \alpha })  \\
&= \frac{1}{2} g^{\mu \alpha } \qty(h_{\alpha \nu , \rho } + h_{\alpha \rho , \nu } - h_{\nu \rho , \alpha })  \marginnote{\(\eta_{\mu \nu }  \) is constant}  \\
&= \frac{1}{2} \eta^{\mu \alpha } \qty(h_{\alpha \nu , \rho } + h_{\alpha \rho , \nu } - h_{\nu \rho , \alpha })   + \mathcal{O}(h^2) \marginnote{We only consider the first order in \(h\)}  \\
&= \frac{1}{2} \qty(h^{\mu }_{\nu , \rho } + h^{\mu }_{\rho , \nu } - \tensor{h}{_{\nu \rho , }^{\alpha }}) + \mathcal{O}(h^2) 
\,.
\end{align}
\end{subequations}

Now, let us look at the Ricci tensor: it is given 
%
\begin{subequations}
\begin{align}
R_{\mu \nu } = R^{\alpha }_{\mu \alpha \nu } 
&= -2 \qty(\Gamma^{\alpha }_{\mu [\alpha , \nu ]}
+ \Gamma^{\beta }_{\mu [\alpha } \Gamma^{\alpha }_{\nu ], \beta })  \\
&= \Gamma^{\alpha }_{\mu \nu , \alpha } - \Gamma^{\alpha }_{\mu \alpha , \nu } + \mathcal{O}(h^2)  \\
&= \frac{1}{2} \qty(\partial_{\alpha } \qty(h^{\alpha }_{\mu , \nu } + h^{\alpha }_{\nu , \mu } - \tensor{h}{_{\mu \nu , }^{\alpha }}) - \partial_{\nu } \qty(h^{\alpha }_{\mu , \alpha } + h^{\alpha }_{\alpha , \mu } - \tensor{h}{_{\mu \alpha ,}^{\alpha }}))  \\
&= \frac{1}{2} \qty(\cancelto{}{h^{\alpha }_{\mu , \nu \alpha }} + h^{\alpha }_{\nu , \mu \alpha } - \tensor{h}{_{\mu \nu , }^{\alpha }_{\alpha }} - \cancelto{}{h^{\alpha }_{\mu , \alpha \nu }} - h^{\alpha }_{\alpha , \mu \nu } + \tensor{h}{_{\mu \alpha ,}^{\alpha }_{\nu }}) \marginnote{Commuting derivatives}  \\
&= - \frac{1}{2} \square h_{\mu \nu } + \frac{1}{2} \qty(h^{\alpha }_{\nu , \mu \alpha } + \tensor{h}{_{\mu \alpha, }^{\alpha }_{\nu }} - h_{,\mu \nu } ) \marginnote{Introduced \(\square = \partial^{\alpha } \partial_{\alpha }\) and  \(h = h^{\alpha }_{\alpha }\)}  \\
&= - \frac{1}{2} \square h_{\mu \nu } + \frac{1}{2} 
\partial_{\mu } \qty(h_{\nu, \alpha  }^{\alpha } - \frac{1}{2} h_{, \nu } ) 
+ \frac{1}{2 } \partial_{\nu } \qty(h_{\mu, \alpha  }^{\alpha } - \frac{1}{2} h_{, \mu }) \marginnote{Split \(h_{, \mu \nu } \) in two, swapped the positions of two contracted indices}
\,,
\end{align}
\end{subequations}
%
which is our final expression. 

For brevity\footnote{Which is the formal way to say that I do not feel like writing it all out.} I omit the proof of the fact that setting \(2 h^{\alpha }_{\nu , \alpha } - h_{, \nu } = 0\) (the harmonic gauge condition) is actually a valid gauge choice, it can be found in the lecture notes. Making this gauge choice, the two terms in parentheses cancel so we find 
%
\boxalign{
\begin{align}
R_{\mu \nu } = - \frac{1}{2} \square h_{\mu \nu }
\,,
\end{align}}
%
which means that, if \(T_{\mu \nu } = 0\), the Einstein Field Equations read \(\square h_{\mu \nu } = 0\), which is precisely the wave equation for a wave propagating with speed \(c\). 

\subsubsection{Gravitational waves polarizations}

We are considering a wave in the form 
%
\begin{align}
h_{\mu \nu } = \exp(i k_{\beta } x^{\beta }) \epsilon_{\mu \nu } = \exp(i \qty(- k t + kz)) \epsilon_{\mu \nu }
\,,
\end{align}
%
for a constant matrix \(\epsilon_{\mu \nu }\) and for \(k_{\mu } = (-k, 0,0,k)\). We have already shown in the exercise before that this satisfies the wave equation. We want to impose the conditions: 
\begin{enumerate}
    \item \(\epsilon_{0 \nu } = 0\);
    \item \(2\partial_{\alpha } h^{\alpha }_{\nu } - \partial_{\nu } h = 0\). 
\end{enumerate}

The first of these also implies \(\epsilon_{\nu 0} = 0\) by symmetry (the symmetry of \(g_{\mu \nu } \) implies the symmetry of \(h_{\mu \nu }\), which in turn implies the symmetry of \(\epsilon_{\mu \nu }\), since the exponential is a scalar).

So, we can write the trace of \(h_{\mu \nu }\) as 
%
\begin{align}
h= \eta^{\mu \nu } h_{\mu \nu } &= \exp(i k_{\beta } x^{\beta } ) \epsilon_{\mu \nu } \eta^{\mu \nu }  \\
&= \exp(i k_{\beta } x^{\beta } ) \epsilon_{ij} \delta^{ij} \marginnote{The components with a 0 vanish, and \(\eta_{ij} = \delta_{ij}\)}
\,,
\end{align}
%
so \(h\) depends on the sum of the diagonal entries of \(\epsilon_{ij}\), which is a constant, we will denote it as \(\epsilon = \epsilon_{ij} \delta^{ij}\). 
Let us now think through the possible values of \(\nu \) in the second condition. If \(\nu =0\) we find: 
%
\begin{align}
2 \partial_{\alpha } h^{\alpha }_{0} - \partial_{0} h = 0
\,,
\end{align}
%
but the first term vanishes since all the components of \(\epsilon_{\mu \nu }\) with an index \(0\) vanish, so the same holds for \(h_{\mu \nu }\). Therefore we get \(\partial_{0} h = 0\), which can be expanded into 
%
\begin{align}
- i k \exp(ik_{\beta } x^{\beta }  ) \epsilon = 0
\,,
\end{align}
%
but \(k \) cannot be 0 for a nontrivial solution, and the exponential always has norm 1, so we must conclude that \(\epsilon = 0\); this implies \(h = 0\).  

Moving on to \(\nu = j \): we get 
%
\begin{align}
0 = \partial_{\alpha } h_{\alpha j} = \partial_{i } h_{ij} = \partial_{3} h_{3 j} = ik \exp(ik_{\beta } x^{\beta } ) \epsilon_{3j}
\,,
\end{align}
%
but, similarly to before, nor \(k\) nor the exponential can be zero, therefore \(h_{3j}=0\), and by symmetry also \(h_{j3}=0\). This means that the matrix \(\epsilon_{\mu \nu }\) looks like 
%
\begin{align}
\epsilon_{\mu \nu } = \left[\begin{array}{cccc}
0 & 0 & 0 & 0 \\ 
0 & \epsilon_{11} & \epsilon_{12} & 0 \\ 
0 & \epsilon_{21} & \epsilon_{22} & 0 \\ 
0 & 0 & 0 & 0
\end{array}\right]
\,,
\end{align}
%
so at this point we are left with two possible degrees of freedom: \(\epsilon_{12} = \epsilon_{21}\), and we found before that \(\epsilon_{\mu \nu }\) must be traceless, which means \(\epsilon_{11} = - \epsilon_{22}\). 

For simplicity I will now write only the smaller \(2 \times 2\) matrix \(\widetilde{\epsilon}_{mn}\), where \(m\) and \(n\) range from 1 to 2. Two possible real matrices which satisfy our conditions are the Pauli matrices \(\widetilde{\epsilon}=   \sigma_{x} \) and \( \widetilde{\epsilon} = \sigma_{z}\): 
%
\begin{align}
\sigma_{x} = \left[\begin{array}{cc}
0 & 1 \\ 
1 & 0
\end{array}\right] \qquad \text{and} \qquad
\sigma_{z} = \left[\begin{array}{cc}
1 & 0 \\ 
0 & -1
\end{array}\right]
\,.
\end{align}

Since we are considering complex superpositions of wave solutions, it should make sense to also include 
%
\begin{align}
\sigma_{y} = \left[\begin{array}{cc}
0 & -i \\ 
i & 0
\end{array}\right]
\,,
\end{align}
%
but I'm not sure whether this is actually done. 


\end{document}
