\documentclass[main.tex]{subfiles}
\begin{document}

\section*{Thu Oct 10 2019}

Last lecture we introduced tensors.

An example of those is the EM tensor \(F_{\mu \nu}\):

\begin{equation}
  F_{\mu \nu} = \left[\begin{array}{cccc}
  0 & E_{x}/c & E_y/c & E_z/c \\ 
  -E_x/c & 0 & -B_x & B_y \\ 
  -E_y/c & B_x & 0 & -B_z \\ 
  -E_z/c & -B_y & B_z & 0
  \end{array}\right]\,,
\end{equation}
%
which, it can be checked, transforms as a \((0,2)\) tensor. Also, we can define the current vector \(j^{\mu} = (c \rho, j^{i})\). Then, the Maxwell equations read:

\begin{equation}
  \partial_{\mu} F^{\mu \nu }= \mu_0 j^{\nu}
  \qquad \text{and} \qquad
  \partial_{[\mu} F_{\nu \rho]}\,.
\end{equation}

They are covariant!

\subsection{Particles in motion}

In Newtonian mechanics, the motion of a particle is described by a function of time \(x^{i} = x^{i}(t)\).

In special relativity, we introduce the concept of \emph{worldline}.
It must be parametrized with respect to some parameter \(\lambda\), such that \(x^{\mu} = x^{\mu}(\lambda)\). A preferred choice for \(\lambda\) is the proper time of the particle, \(\lambda = \tau\).

We then define the 4-velocity:
%
\begin{equation}
  u^\mu = \dv{x ^\mu}{\tau} \,.
\end{equation}

It is a tensor since it is the product of a scalar and a tensor.

Multiplying \(u^\mu u_{\mu}\) we always get \(-c^{2}\), since:

\begin{equation}
  u^{\mu} u_{\mu} = \frac{\dd{x^{\mu}} \dd{x_{\mu}}}{\dd{\tau^{2}}} = -c^2 \frac{\dd{s^{2}}}{\dd{s^2}}
\end{equation}


We can make the expression explicit using \(\dd{\tau} = \gamma \dd{t}\), which gives us \(u^{\mu} = (\gamma c, \gamma v^{i})\).
In the frame of the particle, \(u^{\mu} = (c, 0)\).   

The \emph{four-momentum} of a particle is defined as: 

\begin{equation}
  p^{\mu} = m u^{\mu} = (m \gamma c, m \gamma v^{i})\,.
\end{equation}

The component \(p^{0}\) is \(mc\) at \(v=0\). What does it mean? we can expand it for small \(v\):

\begin{equation}
  \frac{mc}{\sqrt{1 - \frac{v^{2}}{c^{2}}}} \sim
  mc \qty(1 + \frac{v^{2}}{2 c^{2} } )
  = mc + \frac{1}{c} \frac{mv^{2}}{2}\,.
\end{equation}

We get the mass, plus a kinetic energy term: more explicitly, \(cp^0 = mc^{2} + \frac[i]{1}{2} m v^{2}\).

We can rewrite Newton's first law in SR:

\begin{proposition}[Newton I]
A free particle moves with constant \(u^{\mu}\), or 

\begin{equation}
  \dv{u^{\mu}}{\tau} = 0 
\end{equation}
\end{proposition}

To express this in an easier way we introduce the 4-acceleration:

\begin{equation}
  a^{\mu} \defeq \dv{u^{\mu}}{\tau} = \dv[2]{x^{\mu}}{\tau}
\end{equation}

We now with to introduce the concept of a path minimizing proper time. Recall Snell's law, which allows us to relate the angles of incidence of light when passes between one medium to another, if they have different indices of refraction:

\begin{equation}
  \frac{\sin(\theta_{2})}{\sin(\theta_{1})} = \frac{n_1}{n_2 } = \frac{v_2}{v_1 }\,.
\end{equation}

This can be shown to be equivalent to light minimizing the time it takes to move from a point in one medium to a point in the other.

Analogously, saying that a massive particle travels along the worldline which minimizes \(\tau\) is equivalent to Newton's first principle.



\end{document}